Authentication_Tests.v
@@ -1,8 +1,17 @@
 
 Require Import Strand_Spaces Strand_Library Message_Algebra Authentication_Tests_Library.
 
+Definition not_proper_subterm (t:msg) :=  
+  exists (n': node) (L : msg), 
+  t <st L -> t <> L -> r_node n' -> L <[node] n' -> False.
+
 Section TestComponent.
 Variable a t : msg.
-Variable n : node.
+Variable n : node. 
+
+Definition test_component : Prop :=
+  exists (h:msg) (k:Key), t = E h k /\ a <st t /\ t <[node] n /\ not_proper_subterm t.   
 
 End TestComponent.
+Check not_proper_subterm.
+Check test_component.
